model/Non_Failure.thy
@@ -5,8 +5,114 @@ imports
 
 begin
 
-abbreviation(input)
-  "Failed m tr msg \<equiv> ((m, tr, Fail msg) \<in> Traces)"
+lemma final_helper:
+  "\<forall>x. P x \<Longrightarrow> f = g \<Longrightarrow> \<forall>x. P x \<longrightarrow> f x = g x"
+  by simp
+
+lemma nchotomy_helper:
+  "(\<exists>x y. P x y) = (\<exists>t. P (fst t) (snd t))"
+  "(\<forall>x. (\<exists>y. x = f y) \<longrightarrow> Q x) = (\<forall>y. Q (f y))"
+  by auto
+
+lemmas final_simps2[simp] = final_helper[OF monad.nchotomy final_def,
+    simplified imp_disjL all_conj_distrib, simplified nchotomy_helper,
+    simplified]
+
+lemma final_bind_eq:
+  "final (f \<bind> g) = (final f \<and> (case f of Done x \<Rightarrow> final (g x) | _ \<Rightarrow> True))"
+  by (cases f, simp_all add: final_def)
+
+lemma final_bind_TraceD:
+  "(f \<bind> g, tr, x) \<in> Traces \<Longrightarrow> final x \<Longrightarrow>
+    (\<exists>y tr_a tr_b. (f, tr_a, y) \<in> Traces \<and> final y \<and> tr = tr_a @ tr_b \<and>
+        (case y of Done v \<Rightarrow> (g v, tr_b, x) \<in> Traces \<and> final x
+            | _ \<Rightarrow> tr_b = [] \<and> (\<exists>rv. x = monad.map_monad (\<lambda>_. rv) id y)))"
+proof (induct m \<equiv> "f \<bind> g" tr x arbitrary: f g rule: Traces.induct)
+  case Nil
+  then show ?case
+   apply (clarsimp simp: final_bind_eq)
+   apply (intro exI conjI, rule Traces.Nil)
+    apply simp
+   apply (clarsimp split: monad.split_asm simp: Traces.Nil)
+   done
+next
+  case (Step e s'' t s')
+  show ?case using Step.hyps(1-2) Step.prems
+    apply (safe elim!: bind_T_cases)
+     apply (clarsimp simp: final_def[THEN fun_cong, where x="Done _"])
+     apply (erule(1) Traces.Step)
+    apply (drule(1) Step, clarsimp)
+    apply (intro exI conjI, erule(1) Traces.Step)
+      apply simp
+     apply simp
+    apply (clarsimp split: monad.split_asm)
+    done
+qed
+
+definition
+  exec_success_inner :: "bool \<Rightarrow> ('r, 'a, 'e) monad \<Rightarrow> 'r event list \<Rightarrow> bool"
+  where
+  "exec_success_inner exceptions f tr = (\<forall>x. (f, tr, x) \<in> Traces \<longrightarrow> final x \<longrightarrow>
+    (case x of Done _ \<Rightarrow> True | Exception _ \<Rightarrow> exceptions | _ \<Rightarrow> False))"
+
+lemmas exec_success_innerD = exec_success_inner_def[THEN iffD1, rule_format]
+
+lemma exec_success_inner_exc_imp:
+  "exec_success_inner exc f tr \<Longrightarrow> exc \<longrightarrow> exc2 \<Longrightarrow>
+    exec_success_inner exc2 f tr"
+  apply (clarsimp simp: exec_success_inner_def)
+  apply (drule spec, drule(1) mp)
+  apply (clarsimp split: monad.split_asm)
+  done
+
+definition
+  exec_success :: "('r, 'a, 'e) monad \<Rightarrow> ('r event list \<Rightarrow> bool) \<Rightarrow> bool \<Rightarrow> bool"
+  where
+  "exec_success f assum pre = (\<forall>tr. pre \<and> assum tr \<longrightarrow> exec_success_inner False f tr)"
+
+lemmas exec_successI = exec_success_def[THEN iffD2, rule_format]
+
+definition
+  "is_precondition f = True"
+
+lemma exec_success_imp:
+  "exec_success f assum pre \<Longrightarrow>
+    (is_precondition f \<Longrightarrow> pre \<and> assum tr) \<Longrightarrow>
+    exec_success_inner exc f tr"
+  by (clarsimp simp: is_precondition_def exec_success_def
+        exec_success_inner_exc_imp[where exc=False])
+
+lemma exec_success_inner_bind:
+  assumes f: "\<And>tr_a tr_b. tr = tr_a @ tr_b \<Longrightarrow> exec_success_inner exc f tr_a"
+  and g: "\<And>tr_a tr_b v. tr = tr_a @ tr_b \<Longrightarrow> Run f tr_a v \<Longrightarrow> exec_success_inner exc (g v) tr_b"
+  shows "exec_success_inner exc (f \<bind> g) tr"
+  apply (clarsimp simp: exec_success_inner_def)
+  apply (drule(1) final_bind_TraceD, clarsimp)
+  apply (frule f, drule(2) exec_success_innerD)
+  apply (clarsimp split: monad.split_asm)
+  apply (frule(1) g)
+  apply (simp add: exec_success_inner_def)
+  done
+
+lemma exec_success_inner_Choose:
+  "(\<forall>v tr_b. tr = E_choose nm v # tr_b \<longrightarrow> exec_success_inner exc (f v) tr_b) \<Longrightarrow>
+    exec_success_inner exc (Choose nm f) tr"
+  apply (clarsimp simp: exec_success_inner_def)
+  apply (erule Traces_cases, simp_all)
+  apply clarsimp
+  done
+
+lemmas exec_success_inner_inst_simps[simp] =
+    exec_success_inner_def[where f="return _", simplified]
+    exec_success_inner_def[where f="Done _", simplified]
+    exec_success_inner_def[where f="throw _", simplified]
+    exec_success_inner_def[where f="Exception _", simplified]
+
+named_theorems exec_success
+
+lemma assert_exp_exec_success[exec_success]:
+  "exec_success (assert_exp P nm) (\<lambda>_. True) P"
+  by (rule exec_successI, simp add: assert_exp_def)
 
 definition
   regs_ok :: "(string \<times> (('a \<Rightarrow> bool) \<times> 'b)) list \<Rightarrow> 'a event list \<Rightarrow> bool"
@@ -17,58 +123,138 @@ lemma regs_ok_append[simp]:
   "regs_ok regs (xs @ ys) = (regs_ok regs xs \<and> regs_ok regs ys)"
   by (auto simp add: regs_ok_def)
 
-lemma Fail_bind_casesE:
-  assumes f: "Failed (Sail2_prompt_monad.bind m f) t x"
-  assumes early: "\<And>x. Failed m t x \<Longrightarrow> P"
-  assumes late: "\<And>x y tr_a tr_b. Run m tr_a x \<Longrightarrow> Failed (f x) tr_b y \<Longrightarrow> t = tr_a @ tr_b \<Longrightarrow> P"
-  shows "P"
-  apply (rule bind_Traces_cases[OF f])
-   apply (case_tac m'', simp_all)
-    apply (auto elim: late early dest!: sym[where s="Fail _"])
+lemma read_reg_success:
+  "exec_success (read_reg r) (regs_ok regs)
+    (map_of regs (name r) = Some (register_ops_of r))"
+  apply (clarsimp simp: exec_success_inner_def intro!: exec_successI)
+  apply (frule read_reg_non_failure[where f="map_option fst o map_of regs"], simp+)
+   apply (simp add: regs_ok_def)
+  apply auto
   done
 
-lemma Fail_ifE:
-  assumes "Failed (if b then f else g) t msg"
-  obtains "b" and "Failed f t msg" | "\<not>b" and "Failed g t msg"
-  using assms by (auto split: if_splits)
+term "\<forall>c. c \<in> C \<longrightarrow> c \<in> derivable C"
 
-lemma Fail_assert_expE:
-  assumes "Failed (assert_exp P msg') t msg"
-  obtains "\<not> P" and "msg = msg'" and "t = []"
-  using assms by (auto simp: assert_exp_def split: if_splits)
+lemma write_reg_success[exec_success]:
+  "exec_success (write_reg r v) (\<lambda>_. True) True"
+  apply (clarsimp simp: exec_success_inner_def intro!: exec_successI)
+  apply (simp add: write_reg_def)
+  apply (erule Traces.cases)
+   apply (clarsimp simp: final_def[THEN fun_cong, where x="Write_reg _ _ _"])
+  apply (erule T.cases; clarsimp)
+  done
 
-lemmas trace_eqD = arg_cong[where f="\<lambda>m. (m, _, _) \<in> Traces", THEN iffD1]
+definition
+  regs_known :: "(string \<times> (('a \<Rightarrow> bool) \<times> 'b)) list \<Rightarrow> 'a event list \<Rightarrow> bool"
+
+lemma exec_success_inner_foreachM:
+  "(\<forall>x y tr'. x \<in> set xs \<longrightarrow> exec_success_inner exc (f x y) tr') \<Longrightarrow>
+    exec_success_inner exc (foreachM xs y f) tr"
+  apply (induct xs arbitrary: y tr)
+   apply simp
+  apply simp
+  apply (rule exec_success_inner_bind)
+   apply simp
+  apply simp
+  done
 
 lemmas monad_unfolds = and_boolM_def or_boolM_def Let_def[THEN meta_eq_to_obj_eq]
 
-lemma Failed_impossible:
-  "(return x, t, Fail msg) \<in> Traces \<Longrightarrow> P"
-  "(throw x, t, Fail msg) \<in> Traces \<Longrightarrow> P"
-  by auto
+lemmas exec_success_inner_unfold =
+    monad_unfolds[THEN ssubst[where P="\<lambda>m. exec_success_inner _ m _ "]]
 
-lemmas Fail_elims = Fail_bind_casesE
-    Fail_ifE Fail_assert_expE
-    Failed_impossible
-    monad_unfolds[THEN trace_eqD, elim_format]
+definition
+  unat_range_less :: "('a :: len) word \<Rightarrow> nat \<Rightarrow> bool"
+  where
+  "unat_range_less w n = (unat w < n)"
 
-named_theorems failureD
+lemma unat_range_0[simp]:
+  "\<not> unat_range_less w 0"
+  by (simp add: unat_range_less_def)
 
-lemma read_reg_non_failure:
-  "Failed (read_reg r) tr msg \<Longrightarrow> regs_ok regs tr \<Longrightarrow>
-    (map_of regs (name r) \<noteq> Some (register_ops_of r))"
-  by (auto simp: regs_ok_def
-    dest: read_reg_non_failure[where f="map_option fst o map_of regs"])
+lemma unat_range_step[simp]:
+  "n > 0 \<Longrightarrow> w \<noteq> of_nat (n - 1) \<Longrightarrow> unat_range_less w n = unat_range_less w (n - 1)"
+  apply (clarsimp simp: unat_range_less_def)
+  apply (cases "unat w = n - 1", simp_all)
+   apply (cut_tac x=w in unat_lt2p, simp)
+   apply (rule ccontr, erule notE, rule word_unat.Rep_eqD)
+   apply (simp add: unat_of_nat)
+  apply auto
+  done
 
-lemma write_reg_non_failure[failureD]:
-  "Failed (write_reg r v) tr msg \<Longrightarrow> False"
-  by (auto simp: write_reg_def elim: Traces.cases elim!: T.cases)
+lemma to_unat_rangeD[unfolded word_size]:
+  "x \<noteq> of_nat ((2 ^ size x) - 1) \<Longrightarrow> unat_range_less x (2 ^ size x - 1)"
+  apply (drule unat_range_step[rotated])
+   apply simp
+  apply (simp add: unat_range_less_def)
+  done
 
-method non_failure uses rsimps =
-  (determ \<open>auto elim!: Fail_elims dest!: failureD; (auto elim!: Run_elims simp: rsimps)?\<close>)
+ML \<open>
+fun unat_range_intro_tac ctxt = SUBGOAL (fn (t, i) => let
+    val ineqs = Logic.strip_assums_hyp t
+      |> map_filter (try (HOLogic.dest_eq o HOLogic.dest_not o HOLogic.dest_Trueprop))
+      |> filter (can (HOLogic.dest_number o snd))
+    val ineq_tab = Termtab.make_list ineqs
+    val thms = Termtab.dest ineq_tab
+      |> filter (fn (_, xs) => length xs > 2)
+      |> map (fn (t, _) => Var (("z", 0), fastype_of t))
+      |> sort_distinct Term_Ord.fast_term_ord
+      |> map_filter (try (fn x => Drule.infer_instantiate ctxt
+          [(("x", 0), Thm.cterm_of ctxt x)] @{thm to_unat_rangeD}))
+      |> map (Simplifier.full_simplify ctxt)
+   in dresolve_tac ctxt thms i end)
+\<close>
 
-lemma exhaust_helper:
-  "y = max_word \<Longrightarrow> (x \<noteq> y) = (x < y)"
-  "x \<noteq> y - 1 \<Longrightarrow> y \<noteq> 0 \<Longrightarrow> (x < y) = (x < y - 1)"
-  by (auto intro: neq_le_trans dest: inc_le, unat_arith+)
+method_setup unat_range_intro = \<open>Scan.succeed (fn ctxt =>
+    Method.SIMPLE_METHOD (unat_range_intro_tac ctxt 1))\<close>
+
+lemma
+  "(x :: 3 word) \<noteq> 5 \<Longrightarrow> x \<noteq> 6 \<Longrightarrow> x \<noteq> 7 \<Longrightarrow> x \<noteq> 4 \<Longrightarrow> x \<noteq> 3 \<Longrightarrow> x \<noteq> 2 \<Longrightarrow> x \<noteq> 0 \<Longrightarrow> x \<noteq> 1 \<Longrightarrow> False"
+  by (unat_range_intro, simp)
+
+named_theorems exec_success_intro
+
+lemmas exec_success_if[exec_success_intro] =
+    if_split[where P="\<lambda>m. exec_success_inner _ m _", THEN iffD2]
+
+method exec_success_step uses flip = determ \<open>
+      clarsimp intro!: exec_successI exec_success_inner_unfold
+        split del: if_split simp flip: flip
+    | rule conjI exec_success_inner_bind exec_success_intro
+    | (rule exec_success_imp, rule exec_success)
+    | unat_range_intro
+  \<close>
+
+method exec_success uses flip = repeat_new \<open>exec_success_step flip: flip\<close>
+
+lemma success_choose_default[exec_success]:
+  "exec_success (choose_convert_default of_rv x nm) (\<lambda>_. True) (True)"
+  by (clarsimp simp: choose_convert_default_def
+    intro!: exec_successI exec_success_inner_Choose)
+
+lemma success_choose_bool[exec_success]:
+  "exec_success (choose_bool dict nm) (\<lambda>_. True) (True)"
+  by (simp add: choose_bool_def, exec_success)
+
+lemma success_choose_int[exec_success]:
+  "exec_success (choose_int dict nm) (\<lambda>_. True) (True)"
+  by (simp add: choose_int_def, exec_success)
+
+lemma exec_success_bool_of_bitU_nondet[exec_success]:
+  "exec_success (bool_of_bitU_nondet dict b) (\<lambda>_. True) True"
+  by (simp add: bool_of_bitU_nondet_def split: bitU.split, exec_success)
+
+lemma exec_success_of_bits_nondet[exec_success]:
+  "exec_success (bools_of_bits_nondet dict bits) (\<lambda>_. True) True"
+  apply (simp add: bools_of_bits_nondet_def)
+  apply (exec_success | rule exec_success_inner_foreachM)+
+  done
+
+lemma exec_success_bools_of_bits_nondet[exec_success]:
+  "exec_success (of_bits_nondet dict_a dict_b bits) (\<lambda>_. True) True"
+  by (simp add: of_bits_nondet_def, exec_success)
+
+lemma success_choose_from_list[exec_success]:
+  "exec_success (choose_from_list dict nm xs) (\<lambda>_. True) (xs \<noteq> [])"
+  by (simp add: choose_from_list_def, exec_success)
 
 end
